---
layout: blog
title: 公式编辑器
---

$$
E\{\|\hat{\boldsymbol{x}}_{EZF}-\boldsymbol{x}\|^2\}\leq \frac{1}{2}E\{\|\hat{\boldsymbol{x}}_{ZF}-\boldsymbol{x}\|^2\}
$$

$$
y = \begin{bmatrix}
H_1 & H_2 & \cdots & H_K
\end{bmatrix}
\begin{bmatrix}
	x_1 \\
	x_2 \\
	\vdots \\
	x_K	
\end{bmatrix}+n
$$

$$
y_i = y-\begin{bmatrix}
H_1 & \cdots & H_{i-1} & H_{i+1} \cdots & H_K
\end{bmatrix}
\begin{bmatrix}
	x_1 \\
	\vdots \\
	x_{i-1} \\
	x_{i+1} \\
	\vdots \\
	x_K	
\end{bmatrix}
=H_ix_i+n
$$

$$
\begin{aligned}
y&=Hx+n \\
&=\begin{bmatrix} 
h_1 & h_2 & \cdots & h_K
\end{bmatrix}
\begin{bmatrix} 
x_1  \\ 
x_2  \\
\vdots \\
x_K
\end{bmatrix}+n
\end{aligned}
$$ {\end{equation}

$$

$$

![image-20201015215558177](C:\Users\admin\Desktop\公式编辑器.assets\image-20201015215558177.png)
$$
\hat{\mathbf{y}}_i = \mathbf{y}-\sum_{k=1,k\neq i}^{2K}\mathbf{h}_k\hat{x}_t(k)=\mathbf{h}_i\hat{x}_{t+1}(i)
$$

$$
\begin{aligned}
MSE_{ZF}  &=E{\|\boldsymbol{x}-\hat{\boldsymbol{x}}_{ZF}\|_2^2} \\
MSE_{MMSE}&=E{\|\boldsymbol{x}-\hat{\boldsymbol{x}}_{MMSE}\|_2^2}
\end{aligned}
$$

$$
\boldsymbol{y}=\boldsymbol{Hx}+\boldsymbol{n} \\
\boldsymbol{y}=\boldsymbol{HVx}+\boldsymbol{n}
$$

$$
h_{i,j}\in CN(0,1)
$$

